lambda2Gmu/Tests.v
@@ -1,0 +1,54 @@
+Require Import Definitions.
+Require Import TLC.LibLN.
+
+Notation "@ n" := (typ_bvar n) (at level 42).
+Notation "# n" := (trm_bvar n) (at level 42).
+
+Definition id := trm_tabs (trm_abs (@0) (#0)).
+Definition id_typ := typ_all (typ_arrow (@0) (@0)).
+
+Hint Constructors type term wft typing red.
+
+Inductive evals : trm -> trm -> Prop :=
+| eval_step : forall a b c, a --> b -> evals b c -> evals a c
+| eval_finish : forall a, evals a a.
+
+
+Ltac simpl_subst := cbv; try case_if; auto.
+Ltac solve_simple_type := repeat (econstructor; eauto; cbv; try case_if; eauto).
+Ltac fs := exact \{}. (* There must be a better way *)
+
+Lemma well_formed_id :
+  term id
+  /\ type id_typ
+  /\ wft empty empty id_typ.
+  intuition; solve_simple_type.
+  Unshelve. fs. fs. fs. fs.
+Qed.
+
+Lemma well_typed_id : {empty, empty} ⊢ id ∈ id_typ.
+  solve_simple_type.
+Qed.
+
+(* TODO we need an ADT for some Nat numbers type *)
+Definition id_id_app := (trm_app (trm_tapp id id_typ) id).
+Lemma id_of_id_types : {empty, empty} ⊢ id_id_app ∈ id_typ.
+  cbv.
+  repeat (econstructor; eauto).
+  - intros.
+    (* instantiate (1 := _ ==> _). *)
+    instantiate (1 := (@0) ==> @0).
+    solve_simple_type.
+  - intros.
+    instantiate (1 := (@0) ==> @0).
+    solve_simple_type.
+  - simpl_subst.
+Qed.
+
+Ltac crush_eval := repeat (try (apply eval_finish; eauto); econstructor; simpl_subst).
+
+Lemma id_of_id_evals : evals id_id_app id.
+  crush_eval.
+  Unshelve. fs. fs. fs. fs. fs. fs. fs.
+Qed.
+
